
\color{blue}

**Solution**. E\
One way to see (M1) is to calculate in the frequency domain, noting that two stationary Gaussian time series models with the same spectrum are necessarily equal.
$X_n$ is AR(1) and so has spectrum $\sigma^2_\epsilon/|1-a \exp{i\omega}|^2 = \sigma^2_\epsilon/(1+a^2-2a\cos(\omega))$. $\eta_n$ has spectrum $\sigma^2_\eta$, and so $Y_n$ has spectrum
\begin{eqnarray}
\sigma^2_\eta + \frac{\sigma^2_\epsilon}{1+a^2-2a\cos(\omega)}
&=& \frac{\sigma^2_\eta(1+a^2)+\sigma^2_\epsilon - 2a\sigma^2_eta\cos(\omega)}{
1+a^2-2a\cos(\omega)}
\\
&=&
 \sigma^2 \frac{(1+b^2)- 2b\cos(\omega) }{1+a^2-2a\cos(\omega)}
\end{eqnarray}
where $\sigma$ and $b$ solve
\begin{eqnarray}
\sigma^2 (1+b^2) &=& \sigma^2_\eta(1+a^2)+\sigma^2_\epsilon,
\\
\sigma^2 b &=& a\sigma^2_\eta
\end{eqnarray}
Another way to show (M1) is to substitute $X_n = Y_n -\eta_n$ into $X_n = aX_{n-1}+\epsilon_n$ to get
\begin{eqnarray}
Y_n - \eta_n &=& a (Y_{n-1} - \eta_{n-1}) + \epsilon_n,
\\
Y_n - a Y_{n-1} &=& -a\eta_{n-1} + \eta_n + \epsilon_n.
\end{eqnarray}
Notice that this is equivalent to writing
\begin{equation}
Y_n - a Y_{n-1} = \psi \xi_{n-1} + \xi_n,
\end{equation}
where $\var(\xi_n)=\var(\eta_n)+\var(\epsilon_n)$ and $\psi$ is chosen so that
\begin{equation}
\cov(\psi \xi_{n-1},\xi_{n-1}) = \psi \var(\xi_n) = \cov(-a\eta_{n-1}, \eta_{n-1} + \epsilon_{n-1}) = -a \var(\eta_n).
\end{equation}
This calculation checks that the Gaussian model $U_n =  -a\eta_{n-1} + \eta_n + \epsilon_n$ has the same autocovariance as $V_n = \psi\xi_{n-1} + \xi_n$ and so the two models are statisticall indistinguishable.

(M2) is the same set of equations as (M1), as seen by setting $X_n^\prime = \left(\begin{array}{c} X_n \\ \epsilon_n \end{array}\right)$.

(M3) is the ARMA(1,1) case of the LG-POMP representation of a general ARMA model givein in Chapter 11. Specifically, set $X_n = \left(\begin{array}{c} Y_n \\ b \epsilon_n \end{array}\right)$, and see that the process model becomes
\begin{equation}\nonumber
\left(\begin{array}{c} Y_n \\ b \epsilon_n \end{array}\right)
=
\left(\begin{array}{c} a Y_{n-1} + b\epsilon_{n-1} + \epsilon_n \\ b \epsilon_n \end{array}\right).
\end{equation}

\color{black}

